

1. Consider the boundary value problem

$u''(x) = f(x)$, $x < 0 < 1$ and $u(0) = u(1) = 0$ with $f(x) = \frac{1}{x}$. Using $u(x) = \int_0^1 G(s, x) f(s) ds - (\star)$ prove that $u(x) = -x \log(x)$. This show that $u \in C^2(0, 1)$ but $u(0)$ is $f \in C^0([0, 1])$, then u does not belong to $C^0([0, 1])$.

sol: Take

$$G(x, s) = \begin{cases} s(1-x), & 0 \leq s \leq x \\ x(1-s), & x \leq s \leq 1. \end{cases} - (\star\star)$$

Then, by (\star) we have

$$\begin{aligned} u(x) &= \int_0^x s(1-x) \frac{1}{s} ds + \int_x^1 x(1-s) \frac{1}{s} ds \\ &= (1-x)x + x \left(\int_x^1 \frac{1}{s} - 1 \right) \\ &= x(1-x - \ln x - 1 + x) \\ &= -x \ln x. \end{aligned}$$

Hence, we have concluded that $u(x) = -x \ln x$. From $u(1) = 0$ and $\lim_{x \rightarrow 0} u(x) = 0$ which can be proved by L'Hopital's rule, then $u \in C^0([0, 1])$.

2. Clarify the summation by parts formula

$$\sum_{j=0}^{n-1} (w_{j+1} - w_j) v_j = w_n v_n - w_0 v_0 - \sum_{j=0}^{n-1} (v_{j+1} - v_j) w_{j+1},$$

and show that for $v_h \in V_h^0$,

$$(L_h v_h, v_h)_h = h^{-1} \sum_{j=0}^{n-1} (v_{j+1} - v_j)^2.$$

sol:

$$\begin{aligned} RHS &= \sum_{j=0}^{n-1} (w_{j+1} v_j - w_j v_j) \\ &= (w_1 v_0 + w_2 v_1 + \cdots + w_n v_{n-1}) - (w_0 v_0 + w_1 v_1 + \cdots + w_{n-1} v_{n-1}) \\ &= -w_0 v_0 + w_1 (v_0 - v_1) + w_2 (v_1 - v_2) + \cdots + w_{n-1} (v_{n-2} - v_{n-1}) + w_n (v_{n-1} - v_n) + w_n v_n \\ &= w_n v_n - w_0 v_0 - \sum_{j=0}^{n-1} w_{j+1} (v_{j+1} - v_j). \end{aligned}$$

Define $(L_h v)_j = \frac{v_{j+1} - 2v_j + v_{j-1}}{h^2}$. Then

$$\begin{aligned}
(L_h, v_h)_h &= h \sum_{j=1}^{n-1} (L_h v) \cdot v_j = h \sum_{j=1}^{n-1} \frac{v_{j+1} - 2v_j + v_{j-1}}{h^2} v_j \\
&= \sum_{j=1}^{n-1} \frac{v_{j+1} - v_j}{h} v_j - \frac{v_j - v_{j-1}}{h} v_j
\end{aligned}$$

$$\text{by taking } u_{j+1} = v_{j+1} - v_j = \sum_{j=1}^{n-1} (u) \frac{u_{j+1} - u_j}{h} v_j$$

$$\text{by the previous part} = h^{-1} (u_n v_n - u_0 v_0 - \sum_{j=1}^{n-1} u_{j+1} (v_{j+1} - v_j))$$

$$\text{by } u_n = u_0 = 0, = \sum_{j=1}^{n-1} (v_{j+1} - v_j)^2.$$

3. Prove that $G^k(x_j) = hG(x_j, x_k)$, where G is Green's function introduced in $(\star\star)$ and G^k is its corresponding discrete counterpart solution of $(\star\star)$.

sol:

Goal: We want to show that $L_h(hG) = e^k$, and so by $L_h(G^k) = e^k$ which have completed the prove.

Fix x_k is a point. By h is a step as constant number, then $L_h(hG) = h(L_h G)$.

Note that,

$$L_h G(x_k) = \frac{G(x_k + 1, x_k) - 2G(x_k, x_k) + G(x_k - 1, x_k)}{h^2} - (i)$$

For $j \neq k$, by $(\star\star)$, we can see that $G(x_j, x_k)$ is a line, and so for each $l = 0, 1, \dots, k-1$ and $l = k+1, k+2, \dots, n+1$ of the nodes x_l , we have $L_h G = 0$.

For $j = k$, by (i) and define $x_k = kh$ for $k = 0, 1, \dots, n$, then we have the following case:

$$\begin{aligned}
G(x_k, x_k) &= x_k(1 - x_k) = kh(1 - kh) - (ii) \\
G(x_{k+1}, x_k) &= G(x_k + h, x_k) = x_k(1 - x_k - h) = kh(1 - (k+1)h) - (iii) \\
G(x_k - 1, x_k) &= (1 - x_k)x_{k-1} = (1 - kh)(k-1)h - (iv)
\end{aligned}$$

By (i) \sim (iv), then we have

$$L_h G(x_k) = \frac{k(1 - kh + h - 1 + kh) + (1 - kh)(k - 1 - k)}{h} = \frac{1}{h}.$$

Hence, we have $L_h G(hx_j) = 1$.

Therefore we conclude that,

$$L_h(hG) = \begin{cases} 0, & \text{if } j \neq k, \\ 1, & \text{if } j = k. \end{cases}$$